QSemantics.thy
@@ -22,20 +22,16 @@ begin
 
 (* m = partial_state2.ptensor_mat (dims_heap \<vv>) (q \<sigma>) ((Q_domain \<vv>)-(q \<sigma>)) (M::complex mat) (1\<^sub>m (card ((Q_domain \<vv>) - (q \<sigma>))))*)
 (* abbreviation "tensor_vec \<equiv> partial_state2.ptensor_vec" *)
-term  partial_state2.ptensor_mat
 
-definition apply_matrix_sep :: "'q::linorder set \<Rightarrow> ('q, complex) QState \<Rightarrow> complex mat \<Rightarrow> complex vec" 
-  where "apply_matrix_sep sep_vars qs M \<equiv>
+
+definition matrix_sep :: "nat set \<Rightarrow> (complex) QState \<Rightarrow> complex mat \<Rightarrow> complex vec" 
+  where "matrix_sep sep_vars qs M \<equiv>
            let var_d = QState_vars qs in 
-           let v = QState_vector qs in
-           let t = sorted_list_of_set  sep_vars in
-           let l = sorted_list_of_set (var_d - sep_vars) in
-           let vs = sorted_list_of_set var_d in
-           let vs' = (t@l) in
-           let m = partial_state.tensor_mat (list_dims var_d)  {0..<card sep_vars}  
-                                        (M::complex mat) (1\<^sub>m (2^(card (var_d - sep_vars)))) in
-           let q = v.\<^sub>vs \<^sub>\<leadsto> \<^sub>vs' in
-               (m *\<^sub>v q).\<^sub>vs' \<^sub>\<leadsto> \<^sub>vs
+           let var_r = var_d - sep_vars in
+           let v = QState_vector qs in           
+           let m = partial_state2.ptensor_mat sep_vars var_r
+                                        (M::complex mat) (1\<^sub>m (2^(card var_r)))  in           
+               (m *\<^sub>v v)
         "
 
 (* definition alloc_vars :: "'q::linorder set \<Rightarrow> ('q, complex) QState \<Rightarrow> complex vec \<Rightarrow> complex vec"
@@ -56,7 +52,7 @@ definition apply_matrix_sep :: "'q::linorder set \<Rightarrow> ('q, complex) QSt
    let vars_dom' = vars_dom \<union> sep_vars in
     {q. (\<exists>q2. qn = partial_state.tensor_vec (list_dims vars_dom) {0..<card sep_vars} q q2)}" *)
 
-definition measure_vars::"nat \<Rightarrow>  'q::linorder set \<Rightarrow> ('q, complex) QState  \<Rightarrow> (real\<times>complex vec)"
+(* definition measure_vars::"nat \<Rightarrow>  nat set \<Rightarrow> (complex) QState  \<Rightarrow> (real\<times>complex vec)"
   where "measure_vars k  sep_vars qs \<equiv>
    let vars_dom = QState_vars qs in
     let v =   QState_vector qs in
@@ -66,48 +62,108 @@ definition measure_vars::"nat \<Rightarrow>  'q::linorder set \<Rightarrow> ('q,
     let qv = (sorted_list_of_set vars_dom) in
     let qv' = l @ t in 
     let qn = v.\<^sub>qv \<^sub>\<leadsto> \<^sub>qv'  in
-    let mk = partial_state.tensor_mat (list_dims vars_dom) {0..<card sep_vars} (1\<^sub>k (2^(length l))) (1\<^sub>m (2^(length t))) in
-    let qn' =  mk  *\<^sub>v qn in 
+    let mk = partial_state2.ptensor_mat  vars_dom vars (1\<^sub>k (2^(length l))) (1\<^sub>m (2^(length t))) in
+    let qn' =  mk  *\<^sub>v v in 
     let \<delta>k =  Re (((mat_adjoint (mat_of_rows (dim_vec v) [v]) *\<^sub>v qn') $ 0) div vec_norm qn') in    
     let qnprod = ((sqrt \<delta>k)::complex) \<cdot>\<^sub>v qn' in
-       (\<delta>k, qnprod.\<^sub>qv' \<^sub>\<leadsto> \<^sub>qv)" 
+       (\<delta>k, qnprod.\<^sub>qv' \<^sub>\<leadsto> \<^sub>qv)" *)
 
-inductive QSemantics::"'v set \<Rightarrow> ('v,'b,'s,'q::linorder) QConf \<Rightarrow> ('v,'b,'s,'q) QConf \<Rightarrow> bool" 
+definition measure_vars::"nat \<Rightarrow>  nat set \<Rightarrow> (complex) QState  \<Rightarrow> (real\<times>complex vec)"
+  where "measure_vars k  sep_vars qs \<equiv>
+   let vars_dom = QState_vars qs in
+    let v =   QState_vector qs in
+    let vars= (vars_dom - sep_vars) in    
+    let mk = partial_state2.ptensor_mat  vars_dom vars (1\<^sub>k (2^(card vars_dom))) (1\<^sub>m (2^(card vars))) in
+    let qn' =  mk  *\<^sub>v v in 
+    let \<delta>k =  Re (((mat_adjoint (mat_of_rows (dim_vec v) [v]) *\<^sub>v qn') $ 0) div vec_norm qn') in    
+    let qnprod = ((sqrt \<delta>k)::complex) \<cdot>\<^sub>v qn' in
+       (\<delta>k, qnprod)" 
+                                                            
+inductive QSemantics::"'v set \<Rightarrow> ('v,'b,'s) QConf \<Rightarrow> ('v,'b,'s) QConf \<Rightarrow> bool" 
   ("_ \<turnstile> _ \<rightarrow> _" [81,81] 80) for \<Gamma>::"'v set" 
-  where 
-   StackMod:"\<Gamma> \<turnstile> (SMod f, (\<delta>,\<sigma>,\<Q>)) \<rightarrow> (Skip, (\<delta>,f \<sigma>,\<Q>))"
+where 
+\<comment>\<open>SMod  modifies the stack of non-qubits variables \<sigma> with f \<sigma>, where f is a 
+  function modifying the stack\<close>
+   StackMod:"\<Gamma> \<turnstile> (SMod f, Normal (\<delta>,\<sigma>,\<Q>)) \<rightarrow> (Skip, Normal (\<delta>,f \<sigma>,\<Q>))"
+
+\<comment>\<open>QMod modifies the set of qubits of the Quantum State given by q \<sigma> with the 
+  transformation matrix M, any qubit not included in q \<sigma> remains the same\<close>
 
 | QMod:"(q \<sigma>)\<noteq>{} \<Longrightarrow> (q \<sigma>) \<subseteq> (QState_vars \<qq>) \<Longrightarrow> 
-         \<qq>' = apply_matrix_sep (q \<sigma>) \<qq> m \<Longrightarrow>
-         \<Gamma> \<turnstile> (QMod M q, (\<delta>,\<sigma>,(\<vv>,\<qq>))) \<rightarrow> (Skip, (\<delta>, \<sigma>,(\<vv>,QState(QState_vars \<qq>, list_of_vec  \<qq>'))))"
+         \<qq>' = matrix_sep (q \<sigma>) \<qq> m \<Longrightarrow>
+         \<Gamma> \<turnstile> (QMod M q, Normal (\<delta>,\<sigma>,(\<vv>,\<qq>))) \<rightarrow> (Skip, Normal (\<delta>, \<sigma>,(\<vv>,QState(QState_vars \<qq>, list_of_vec  \<qq>'))))"
 
- | Alloc:"q' \<notin> (dom_q_vars \<vv>) \<Longrightarrow> q'_addr \<in> new_q_addr (e \<sigma>) \<vv> \<Longrightarrow> 
+\<comment>\<open>QMod fails if the set of qubits to be modified is not included in the quantum state\<close>
+| QMod_F:"\<not> ((q \<sigma>) \<subseteq> (QState_vars \<qq>)) \<Longrightarrow>          
+         \<Gamma> \<turnstile> (QMod M q, Normal (\<delta>,\<sigma>,(\<vv>,\<qq>))) \<rightarrow> (Skip, Fault)"
+
+\<comment>\<open>Alloc takes a normal variable "q" representing the variable where the index to the qubits is store
+   an function e from the state \<sigma> to a natural number representing the number of qubits to allocate
+  and an initialization value for the allocated qubits 
+
+
+  We will require that a program is well formed, meaning that the types are correct.
+  A call to Alloc is well formed if the type of q is a natural number\<close>
+
+| Alloc:"q' \<notin> (dom_q_vars \<vv>) \<Longrightarrow> q'_addr \<in> new_q_addr (e \<sigma>) \<vv> \<Longrightarrow>
           \<vv>' = \<vv>(q' := q'_addr)  \<Longrightarrow> length (v \<sigma>) = (e \<sigma>) \<Longrightarrow> \<sigma>' = set_value \<sigma> q (nat_to_typ q') \<Longrightarrow>                    
-          \<Gamma> \<turnstile> (Alloc q e v, (\<delta>,\<sigma>,(\<vv>,\<qq>))) \<rightarrow> (Skip, (\<delta>, \<sigma>',(\<vv>',\<qq> + QState (q'_addr,(v \<sigma>)) )))"
+          \<Gamma> \<turnstile> (Alloc q e v, Normal (\<delta>,\<sigma>,(\<vv>,\<qq>))) \<rightarrow> (Skip, Normal (\<delta>, \<sigma>',(\<vv>',\<qq> + QState (q'_addr,(v \<sigma>)) )))"
 
- | CondTrueQ:"\<sigma>\<in>b  \<Longrightarrow> \<Gamma> \<turnstile> (IF b c1 c2, (\<delta>,\<sigma>,\<Q>)) \<rightarrow> (c1, (\<delta>,\<sigma>,\<Q>))"
+\<comment>\<open>Alloc will fail if the length of the initial value is not equal to the number of qubits allocated \<close>
 
- | CondFalseQ:"\<sigma>\<notin>b  \<Longrightarrow> \<Gamma> \<turnstile> (IF b c1 c2, (\<delta>,\<sigma>,\<Q>)) \<rightarrow> (c2, (\<delta>,\<sigma>,\<Q>))"
+
+ | Alloc_F:"length (v \<sigma>) \<noteq> (e \<sigma>) \<Longrightarrow>                    
+          \<Gamma> \<turnstile> (Alloc q e v, Normal (\<delta>,\<sigma>,(\<vv>,\<qq>))) \<rightarrow> (Skip, Fault)"
+
+\<comment>\<open>the conditional, while, and seq statements follow the standard definitions\<close>
+
+| CondTrueQ:"\<sigma>\<in>b  \<Longrightarrow> \<Gamma> \<turnstile> (IF b c1 c2, Normal (\<delta>,\<sigma>,\<Q>)) \<rightarrow> (c1, Normal (\<delta>,\<sigma>,\<Q>))"
+
+ | CondFalseQ:"\<sigma>\<notin>b  \<Longrightarrow> \<Gamma> \<turnstile> (IF b c1 c2, Normal (\<delta>,\<sigma>,\<Q>)) \<rightarrow> (c2, Normal (\<delta>,\<sigma>,\<Q>))"
 
  | WhileTruec: "s\<in>b \<Longrightarrow> 
-                \<Gamma>\<turnstile> (While b c,(\<delta>,\<sigma>,\<Q>)) \<rightarrow> (Seq c (While b c),(\<delta>,\<sigma>,\<Q>))"
+                \<Gamma>\<turnstile> (While b c,Normal (\<delta>,\<sigma>,\<Q>)) \<rightarrow> (Seq c (While b c), Normal (\<delta>,\<sigma>,\<Q>))"
 
  | WhileFalsec: "s\<notin>b \<Longrightarrow> 
-                 \<Gamma>\<turnstile> (While b c,(\<delta>,\<sigma>,\<Q>)) \<rightarrow> (Skip,(\<delta>,\<sigma>,\<Q>))"
+                 \<Gamma>\<turnstile> (While b c, Normal (\<delta>,\<sigma>,\<Q>)) \<rightarrow> (Skip, Normal (\<delta>,\<sigma>,\<Q>))"
 
 | Seqc:"\<lbrakk>\<Gamma> \<turnstile> (C1, \<sigma>) \<rightarrow> (C1', \<sigma>')\<rbrakk> \<Longrightarrow> \<Gamma> \<turnstile> (C1;C2, \<sigma>) \<rightarrow> (C1'C2, \<sigma>')"
 
 | SeqSkipc: "\<Gamma>\<turnstile> (Skip;C2,\<sigma>) \<rightarrow> (C2, \<sigma>)"
 
-| Dispose: "\<vv> (q \<sigma>) \<noteq> {} \<Longrightarrow> \<vv>' = \<vv>((q \<sigma>):={}) \<Longrightarrow> \<qq>1 ## \<qq>2  \<Longrightarrow> 
-            \<vv> (q \<sigma>) = QState_vars \<qq>2 \<Longrightarrow> \<qq> =   \<qq>1 +  \<qq>2 \<Longrightarrow>            
-             \<Gamma> \<turnstile> (Dispose q, (\<delta>,\<sigma>,(\<vv>,\<qq>))) \<rightarrow> (Skip,(\<delta>,\<sigma>,(\<vv>',\<qq>1)))"
+\<comment>\<open>Dispose takes an expression from the stack to a natural number and removes those qubits
+  from the quantum state if they are not entangled with the rest of qubits in the current
+  Quantum state. The entanglement condition is that it is possible to find a vector \<qq>1 such that
+  \<qq> =  \<qq>' +  \<qq>''\<close>
+
+| Dispose: "\<vv> (q \<sigma>) \<noteq> {} \<Longrightarrow> \<vv>' = \<vv>((q \<sigma>):={}) \<Longrightarrow> \<qq>' ## \<qq>''  \<Longrightarrow> 
+            \<vv> (q \<sigma>) = QState_vars \<qq>'' \<Longrightarrow> \<qq> =   \<qq>' +  \<qq>'' \<Longrightarrow>            
+             \<Gamma> \<turnstile> (Dispose q, Normal (\<delta>,\<sigma>,(\<vv>,\<qq>))) \<rightarrow> (Skip,Normal (\<delta>,\<sigma>,(\<vv>',\<qq>')))"
+
+\<comment>\<open>Dispose dispose will fail if it is not possible to find such states \<qq>',  \<qq>''\<close>
+
+
+| Dispose_F: "\<nexists>\<qq>' \<qq>'. \<vv> (q \<sigma>) \<noteq> {} \<and> \<vv> (q \<sigma>) = QState_vars \<qq>'' \<and> 
+               \<qq> =   \<qq>' +  \<qq>'' \<and> \<qq>' ## \<qq>'' \<Longrightarrow>
+               \<Gamma> \<turnstile> (Dispose q, Normal (\<delta>,\<sigma>,(\<vv>,\<qq>))) \<rightarrow> (Skip,Fault)"
+
+\<comment>\<open>Measure measures the value of the set of qubits given by q \<sigma> and it stores the result in 
+  the stack variable v. Similar to allocate, we will require that the construct is well formed
+ and that the type of v is a real number\<close>
 
 | Measure: "q \<sigma> \<subseteq> (QState_vars \<qq>) \<Longrightarrow> 
             (\<delta>k, \<qq>') = measure_vars k (q \<sigma>) \<qq> \<Longrightarrow>
             \<delta>k > 0 \<Longrightarrow> \<delta>' = \<delta> * \<delta>k \<Longrightarrow> 
-            \<Gamma> \<turnstile> (Measure v q, (\<delta>,\<sigma>,(\<vv>,\<qq>))) \<rightarrow> (Skip,(\<delta>',\<sigma>,(\<vv>,QState(Q_domain \<vv>', list_of_vec  \<qq>'))))" 
- 
+            \<Gamma> \<turnstile> (Measure v q, Normal (\<delta>,\<sigma>,(\<vv>,\<qq>))) \<rightarrow> (Skip,Normal (\<delta>',\<sigma>,(\<vv>,QState(Q_domain \<vv>', list_of_vec  \<qq>'))))" 
+
+\<comment>\<open>Since Measure access to the values of the qubits given by q \<sigma> as QMod, 
+  Measure will similarly fail if the set of qubits to be mesured does not
+  belong to the set of allocated qubits\<close>
+
+| Measure_F: "\<not> (q \<sigma> \<subseteq> (QState_vars \<qq>)) \<Longrightarrow>  
+            \<Gamma> \<turnstile> (Measure v q, Normal (\<delta>,\<sigma>,(\<vv>,\<qq>))) \<rightarrow> (Skip, Fault)" 
+
+
 (* | Dispose: "\<vv> (q \<sigma>) \<noteq> {} \<Longrightarrow> \<vv>' = \<vv>((q \<sigma>):={}) \<Longrightarrow> \<qq>1 ## \<qq>2  \<Longrightarrow> 
             \<vv> (q \<sigma>) = QState_vars \<qq>2 \<Longrightarrow> \<qq> =   \<qq>1 +  \<qq>2 \<Longrightarrow>
             \<qq>' \<in> dispose_vars (\<vv> (q \<sigma>)) \<qq> \<Longrightarrow>
